src-lite/wl_properties.v
@@ -3,6 +3,30 @@ Require Import decl_worklist.
 Require Import transfer.syntax.
 Require Import transfer.properties.
 
+Require Import decl.notations.
+Require Import Equality.
+Require Import ln_utils.
+
+Lemma solve_wf : forall Γ, ⪧ Γ → ⫦ ⌊ Γ ⌋.
+Proof.
+  induction 1; simpl.
+  - admit.
+  - admit.
+  - admit.
+  - admit.
+  - admit.
+  - admit.
+  - admit.
+Admitted.
+
+Lemma solve_prefix : forall Γ1 Γ2,
+    ⪧ Γ1 ⫢ Γ2 → ⪧ Γ1.
+Proof.
+  intros.
+  dependent induction H.
+  - destruct Γ1; destruct Γ2; solve [auto | inversion x].
+  - admit.
+Admitted.
 
 Theorem wl_sound : forall Γ',
     ⪧′ Γ' → exists Γ Θ, nil ⊩ Γ' ⟿ Γ ⫣ Θ ∧ ⪧ Γ.
@@ -14,5 +38,126 @@ Proof.
   (* var *)
   - admit.
   (* num *)
+  - destruct IHwl_step as (Γ0 & Θ & Inst & DeclSolve).
+    apply inst_wl_split in Inst as (Γ1 & Γ2 & Θ0 & -> & Inst1 & Inst2).
+    pick fresh x for (fv_worklist c `union` fv_ss Θ).
+    rewrite (subst_worklist_intro x) in Inst2; auto.
+    assert (exists Θ', Θ0 ;; Θ' = Θ) as (Θ' & <-)
+        by eauto using inst_wl_ss_extend.
+    eapply inst_wl_rev_subst with (e := be_int) in Inst2
+        as (c' & Θ'' & <- & <- & Inst2).
+    exists (Γ1 ⊨ be_num n ⇒ close_dworklist_wrt_bexpr x c'). exists (Θ0 ;; Θ'') (* todo *).
+    split.
+    + apply instwl_cons with Θ0.
+      * auto.
+      * eapply instw_infer; eauto. intros.
+        rewrite (subst_worklist_intro x).
+        rewrite (subst_dworklist_intro x).
+        apply inst_wl_rename.
+        rewrite open_dworklist_wrt_bexpr_close_dworklist_wrt_bexpr. auto.
+        all: admit.
+    + eapply dst_infer with be_int.
+      * admit.
+      * now rewrite <- subst_dworklist_spec.
+    + admit.
+    + admit.
+    + admit.
+  (* int *)
+  - admit.
+  (* star *)
+  - admit.
+  (* star check *)
+  - admit.
+  (* bot check *)
+  - admit.
+  (* app *)
+  - f1 <: f2 ⇒ A
+    A . e ⇒ B
+    destruct IHwl_step as (Γ' & Θ & Inst & Solve).
+    dependent destruction Inst.
+    dependent destruction H0.
+    dependent destruction Solve.
+
+    admit.
+  (* lambda check *)
+  - admit.
+  (* pi *)
+  - inst_cofinites_with_new.
+    inst_cofinites_with_new.
+    inst_cofinites_with_new.
+    destruct H0 as (Γ0 & Θ & Inst & Solve).
+    dependent destruction Inst.
+    dependent destruction Inst.
+    dependent destruction Inst.
+    dependent destruction Inst.
+    dependent destruction H0. dependent destruction H0.
+    dependent destruction H4. dependent destruction H4.
+    apply inst_wl_split in Inst as (Γ1 & Γ2 & Θ' & -> & Inst1 & Inst2).
+    dependent destruction Inst1.
+    pick fresh x' for all.
+    rewrite (subst_worklist_intro x) in Inst2.
+    assert (exists Θ'0, Θ' ; x1 ≔ ⧼k0⧽ ;; Θ'0 = Θ) as (Θ'0 & <-)
+        by eauto using inst_wl_ss_extend.
+    eapply inst_wl_rev_subst with (e := ⧼k0⧽') in Inst2
+        as (c_' & Θ'0' & <- & <- & Inst2).
+    exists (Γ0 ⊨ be_pi A0 (close_bexpr_wrt_bexpr x e1) <: be_pi A4 (close_bexpr_wrt_bexpr x e0) ⇒ (close_dworklist_wrt_bexpr x c_')), nil. split.
+    all: admit.
+    (*
+    + admit.
+    + eapply dst_infer with (⧼k0⧽').
+      dependent destruction H10.
+      dependent destruction H10.
+      assert (A5 = ⧼k0⧽') as -> by admit.
+      assert (e4 = e5) as -> by admit.
+      all: admit.
+    *)
+  (* bind check *)
+  - admit.
+  (* forall L *)
+  - admit.
+  (* forall R *)
+  - admit.
+  (* forall LR *)
+  - admit.
+  (* castdn *)
+  - admit.
+  (* castup *)
+  - admit.
+  (* anno *)
+  - admit.
+  (* ex infer *)
+  - admit.
+  (* ex inst l *)
+  - admit.
+  (* ex inst r *)
+  - admit.
+  (* app infer rec *)
+  - admit.
+  (* app infer base *)
+  - admit.
+  (* app infer ex *)
+  - admit. (* todo, fix the rule *)
+  (* gen-red base *)
+  - admit.
+  (* gen-red rec *)
+  - admit.
+  (* kind-ex *)
+  - admit.
+  - admit.
+  - admit.
+  - admit.
+  (* check *)
+  - admit.
+  (* compatible *)
+  - admit.
+  - admit.
+  - admit.
+  - admit.
+  - admit.
+  (* var binding *)
+  - admit.
+  (* ex binding *)
+  - admit.
+  (* kex binding *)
   - admit.
 Admitted.
